#+TITLE: How to prove it: a structured approach
#+ROAM_KEY: cite:velleman2019prove
* TODO Notes
:PROPERTIES:
:Custom_ID: velleman2019prove
:NOTER_DOCUMENT: /home/mvmaciel/Drive/Org/pdfs/velleman2019prove.pdf
:AUTHOR: Velleman, D. J.
:JOURNAL:
:DATE:
:YEAR: 2019
:DOI:
:URL:
:END:



* Why am I reading this/ Where this might be useful/Which project or idea that I already have will benefit from this and how?
Learn math lol


* Struct questions

** What are the main concepts of the text?
*** Chap 1-2 :ATTACH:
:PROPERTIES:
:ID:       86e765fd-5b51-40a0-a9d8-551a57235cdd
:END:
- The laws of conjunction/disjunction (which can be proved using truth tables):
  [[attachment:_20210104_181532screenshot.png]]

- The laws of tautology and contradiction

[[attachment:_20210104_182447screenshot.png]]
- The *symmetric difference* \(A \triangle B \)
  [[attachment:_20210104_192435screenshot.png]]
- How does one translate from logic to sets?
  - By using *truth sets*
    [[attachment:_20210104_192708screenshot.png]]
- The *conditional laws*
  [[attachment:_20210105_103902screenshot.png]]
- One useful equivalence is  \(P \iff Q = (P \land Q) \lor ( \neg P \land \neg Q) \)
- Be careful with biconditional equivalences!! Try to spell them, since they are tricky. Page 54 shows some of them
- The *quantifier negation laws*
  [[attachment:_20210105_111322screenshot.png]]
- *Uniqueness* is formalized as following : \(\exists !x P(x) = \exists x (P(x) \land \neg \exists y (P(y) \land y\neq x))\)
- Notice that universal conditionals are *vacuously true* if the universe of the antecedent is \(\emptyset\)  .
- Notice that \(\exists x \in A P(x) = \exists x ( \in A \land P(x))\) and that  \(\forall x \in A P(x) = \forall x (x \in A \rightarrow P(x))\)
- Notice that \(x \in \{n^2 | n \in \mathbb{N}\} = \exists n \in \mathbb{N}(x = n^2)\)
- The *universal quantifier distributes over conjunction*: \( \forall x (E(x)
  \land T(x)) = \forall x E(x) \land \forall x T(x) \) while the *existential
  quantifier distributes over disjunction*: \(\exists x (P(x) \lor Q(x)) =
  \exists x P(x) \lor \exists x Q(x)\)
- *Indexed family* : \( x \in \{ x_i | i \in I\} = \exists i \in I(x = x_i) \)
- The generalized definitions of intersection and union are actually non-trivial:
  [[attachment:_20210105_135306screenshot.png]]
  + Where families are sets constituted of other sets
  + Intersection = the contrapositive and turning into disjunction is easier to grasp \(\{x| \forall A (x \in A \lor A \notin F)\}\)
  + It is even easier to understand using indexed families. Let \(F = \{A_i | i \in I\}\) then:
    - \(\cap F = \cap _{i \in I}A_i =\{x | \forall i \in I (x \in A_i)\}\)   (x is in all indexes of the family)
    - \[ \cup F = \cup_ {i \in I} A_i = \{x | \exists i \in I (x \in A_i ) \} \] (x is there because it is in some index)
*** Chap 3 - Proof strategies
- Proofs are games of folding *givens* towards *goals*
- *Proving goals of the form*:
  - \(\neg P\):
    a. Reexpress as a positive statement
    b. Use proof by contradiction
  - \(P \to Q\):
    a. Assume P and prove Q (*modus ponens*)
    b. Prove the contrapositive: assume Q is false and prove that P is false (*modus tollens* )
  - \(P \land Q\):
    - Prove P and Q separately. Treat this as two separate goals
  - \(P \lor Q\):
    a. Assume P is false and prove Q, or assume Q is false and prove P
    b. Use proof by cases
  - \( P \iff Q\)
    a. Prove the conditionals separately
  - \(\forall x P(x)\)
    a. Let \(x\) stand for an arbitrary object and prove \(P(x)\)
  - \(\exists P(x)\)
    a. Find a value of \(x\) that makes \(P(x)\) true. Prove \(P(x)\) for this value of \(x\)
  - \(\exists !x P(x)\)
    a. Prove \(\exists P(x)\) and \(\forall y \forall x ((P(y) \land P(z)) \to y = z)\)
    b. Prove \(\exists x ( P(x)  \land \forall y (P(y) \to y = x)  ) \)
  - \(\forall n \in \mathbb{N} P(n)\)
    a. Mathematical induction: Prove base case and \(\forall n \in \mathbb{N} (P(n) \to P(n+1))\) (the induction step)
    b. Strong induction: \(\forall n \in \mathbb{N} [(\foall k < n P(k)) \to P(n)]\)
- *When using a given of the form*:
  - \(\neg P\):
    a. Reexpress as a positive statement
    b. If proving by contradiction, try to prove P
  - \(P \to Q\)
    a. If given / proven P then Q follows
    b. Use the contrapositive: if given / proven Q is false, then \(\neg P\) ensues
  - \(P \land Q\):
    a. Treat as two givens
  - \(P \lor Q\):
    a. Use proof by cases. Assume P is true in case 1. Assume Q is true in case 2.
    b. If given / proven that \(\neg P\) then Q follows. THe same if Q is false
  - \(\forall x P(x)\)
    a. Plug in any value \(a\) and conclude that \(P(a)\) is true
  - \(\exists P(x)\)
    a. Introduce a new variable \(x_0\) that stands for a particular object for which \(P(x_0)\) is true
  - \(\exists !x P(x)\)
    a) Introduce a new variable \(x_0\) that stands for a particular object for
      which \(P(x_0)\) is true. Also, you may assume that \(\forall y (P(y) \to y=x_0)\)
- *General proofs techniques*
  - Proof by contradiction
  - Proof by cases
*** Chap 4 - Relations :ATTACH:
:PROPERTIES:
:ID:       f5bee330-1195-4cce-9d12-8779e2fb8bda
:END:
- *Cartesian Product*:
  \(A \times B = \{(a,b) \text{  } | \text{  } a \in A \text{ and } b \in B\}\)
- The Cartesian Product is fundamental because it is needed to define the truth set for statements containing two free variables !!!!!!
  + Truth set of \(P(x,y) = \{(a,b) \in A \times B \text{  } | \text{  } P(a,b)\}\)
- A *Relation* is defined as \(R \subseteq A \times B\)
- The *Domain* is defined as \(\text{Dom}(R) = \{a \in A \; | \,  \exists b \in B ((a,b) \in R)\}\)
- The *Range* is defined as  \(\text{Ran}(R) = \{b \in B \; | \exists a \in A ((a,b) \in R)\}\)
- The *inverse* is defined as \(R^{-1} = \{(b,a) \in B \times A \; | \,  (a,b) \in R \}\)
- The *composition* is defined as
  - \(S \circ R = \{(a,c) \in A \times C \; | \, \exists b \in B ((a,b) \in R \text{ and } (b,c) \in S)\}\)
- A relation is *reflexive on \(A\)* if \(\forall x \in A((x,x) \in R)\)
- A relation is *symmetric* if \(\forall x \in A \forall y \in A (xRy \to yRx)\)
- A relation is *transitive* if \(\forall x \in A \forall  z \in A ((xRy \land yRz) \to xRz)\)
- Some useful facts:
  - R is reflexive iff \(i_A \subseteq R \)
  - R is symmetric iff \(R = R^{-1}\)
  - R is transitive iff \(R \circ R \subseteq Let\)
- \(R \subseteq A \times A\). It is *antisymmetric* if \(\forall x,y \in A ((xRy \land yRx) \rightarrow x = y)\)
- \(R \subseteq A \times A\). It is a *partial order* if it is reflexive, transitive and antisymmetric. It is a *total order* if it is a partial order and it is also total: \(\forall x,y \in A(xRy \lor yRx)\) .
- If R is a partial order on A, \(B \subseteq A\) and \(b \in B\) there are two important concepts:
  - b is the *R-smallest element* of \(B\) if \(\forall x \in B (bRx)\)
  - b is the *R-minimal element* of \(B\) if \(\neg \exists x \in B(xRb \land x \neq b)\) which is the same as saying that \(\forall x \in R ((x,b) \in R \rightarrow x = b)\)
  - b is the *R-largest element* of \(B\) if \(\forall x \in B (xRb)\)
  - b is the *R-maximal element* of \(B\) if \(\neg \exists x \in B(bRx \land x \neq b)\) which is the same as saying that \(\forall x \in R ((b,x) \in R \rightarrow x = b)\)
- Those definitions are really important in decision theory (pareto frontier and so on )
- Some useful properties of smallest/minimal elements:
  [[attachment:_20210114_161955screenshot.png]]
- It is common to apply the notion of smallest element to sets. So one works with power sets instead of simple sets, and the smallest element, given a relation (or property),  will be the one which is a subset of all other sets which also have this property.
- *Lower bounds*  and *upper bounds* are also useful concepts closely related to smallest and largest elements:
  - Suppose R is a partial order on A; \(B \subseteq A\) and \(a \in A\)
  - \(a\) is a *lower bound* for B if \(\forall x \in B (aRx)\)
  - \(a\) is an *upper bound* for B if \(\forall x (xRa)\)
  - Note that a lower bound for B need not be an element of B !!!!!
- Other important concepts are the ones of *least upper bound* and *greatest upper bound*
  [[attachment:_20210114_174751screenshot.png]]



* Exercises
- Page 81 exercise 1.d
** Section 3.3
- 2:
  + Goal
    - \(A
      \cap
       B
        \setminus
         C =
          \emptyset
          \to
          A \cap B
           \subseteq
            C\)
  + Proof
    - Suppose \(A \cap B \setminus C = \emptyset\). From the disjoint we know
      that either \(x \notin A\) or \(x \notin B\) or \(x \in C\). Now suppose \(x \in A \cap B \) . Then, necessarily, \(x \in C\). Thus if \(A \cap B \setminus C = \emptyset\) then  \(A \cap B \subseteq C\) .
- 3:
  - Goal:
    - \(A \subseteq B\setminus C \to A \cap C = \emptyset\)
  - Proof:
    - Suppose \(A \subseteq B\setminus C \). We may translate \(A \cap C = \emptyset\) as saying that if \(x \in A\) then \(x \notin C\) . Well, suppose \(x \in A\). Then from \(A \subseteq B\setminus C \) we know that it is an element of B, but not of C. Thus we have proved that \(A \cap C = \emptyset \)
- 4:
  - Given:
    - \(A \subseteq \mathcal{P}(A)\)
  - Goal:
    - \(\mathcal{P}(A) \subseteq \mathcal{P}(\mathcal{P}(A))\)
  - Suppose \(X \in \mathcal{P}(A)\). Then  \(X \subseteq A\) which leads us to recognize, through \(A \subseteq \mathcal{P}(A)\),  that an element \(x \in X\)  is also an element of \(\mathcal{P}(A)\), that is \(X \subseteq \mathcal{P}(A) = X \in \mathcal{P}(\mathcal{P}(A))\) . This means that if \(X \in \mathcal{P}(A)\) then \(X \in \mathcal{P}(\mathcal{P}(A))\) . Hence, \(\mathcal{P}(A) \subseteq \mathcal{P}(\mathcal{P}(A))\).
- 6:
  - Goals:
    - \(x \neq 1 \iff \text{ there is a number y s.t. } {{y + 1} \over {y-2}} = x\)
  - Solve for y. \(y = {(2x + 1) \over (1 - x )}\) . Iff \(x \neq 1\) y exists.
- 7:
  - Let \(y =  {{x + \sqrt{x^2 - 4}} \over 2 }\). Substitute it in \(y + {1 \over y} = x \).
- 8:
  - Goal:
    - \( A \in \mathcal{F}::Set(Set) \to A \subseteq \cup\mathcal{F}\)
  - Proof:
    Suppose \(A \in \mathcal{F}\). Now suppose \(x \in A\) . By the definition of \(\cup \mathcal{F}\) we have that \(x \in \mathcal{F}\), from which follows that \(A \subseteq \mathcal{F}\) and, hence, \( A \in \mathcal{F}::Set(Set) \to A \subseteq \cup\mathcal{F}\)
- 9:
  - Goal:
    - \( A \in \mathcal{F}::Set(Set) \to  \cap\mathcal{F} \subseteq A\)
    - It is easier to prove the contrapositive. Assume \( \cap\mathcal{F} \not\subseteq A\) . This means that there is an \(x\) s.t. \(x\in \cap \mathcal{F}\) and \(x \notin A\) . From the definition of intersection we know that \(x\) must be an element of all the elements of \(\mathcal{F}\) . This is only possible if \(A \notin F\).
    - Maybe it was easier to prove directly kkkkkkk
- 14:
  - Suppose \(x \in \cup_{i \in I}
     \mathcal{P}(A_i)
     \). Then there is an index s.t. \(x \subseteq A_i\) . Now suppose \(y \in x\). From \(x \subseteq A_i\) we know that \(y \in A_i\). Thus, \( y\in \cup_{i \in I}(A_i)\). Since y is arbitrary \(x \subseteq \cup_{i \in I}(A_i) \), which is the same as \(x \in
     \mathcal{P}(\cup_{i \in I} (A_i))\).
-
** Section 3.5
- 1:
  + Goal: \(A \cap (B \cup C) \subseteq (A \cap B) \cup C\)
  + Suppose \(x \in A \cap (B \cup C)\). Since \(x \in B \cup C\) either \(x \in B\) or \(x \in C\) we have:
    - Case 1: Assume \(x \in B\). Then \(x \in A \cap B\) from which we conclude that \(x \in (A \cap B) \cup C\)
    - Case 2: Assume \(x \in C\). Then it is clear that \(x \in (A \cap B) \cup C\)
    Thus, \(A \cap (B \cup C) \subseteq (A \cap B) \cup C\) .
- 2:
  - Goal: \( (A \cup B) \setminus C
    \subseteq
    A \cup (B \setminus C)
    \)
  - Suppose \(x \in (A \cup B) \setminus C\) . Then \(x \notin C\) and either \(x \in A\) or \(x \in B\).
    - Case 1: Assume \( x \in A\). Clearly \(x \in     A \cup (B \setminus C) \)
    - Case 2: Assume \(x \in B\). Then \( x \in B \setminus C\) and, subsequently, \(x \in A \cup (B \setminus C)\)
- 3:
  - Goal: \(A \setminus (A \setminus B) = A \cap B\)
  - Proof:
               \[\begin{aligned}x \in A \setminus  (A \setminus B) = \\
    x \in A \land (x \notin (A \setminus B))  = \\
    x \in A \land  (x \notin A \lor (x \in B)) = \\
    x \in A \land (x \in A \to x \in B)  = \\
    x \in A \land x \in B = \\
    x \in A \cap B
    \end{aligned}\]
- 4:
  - Goal: \(A \subseteq B\)
  - Given:
    + \(A \cap C \subseteq B \cap C\)
    + \(A \cup C \subseteq B \cup C\)
  - Proof
    - Suppose \(x \in A\). Then \(x \in B \cup C\), since \(x \in A \cup C\). Now either \(x \in B \) or \(x \in C\). If \(x \in B\) the proof is done. Now suppose \(x \in C\). Then it is also an element of \(A \cap C\) and hence of \(B\cap C\). Thus, \(x \in B\). Since x was arbitrary, \( A \subseteq B\).
- 5
  - Goal: \(A \triangle B \subseteq A \to B \subseteq A\)
  - Suppose \(A \triangle B \subseteq A\). Now either \(x \in B \to x \in A\)  or \(x \in A \to x \in B\). The first case is trivial. The second can be proven by using the contrapositive.
- 6
  - Goal: \(A \cup C \subseteq B \cup C \iff
    A \setminus C \subseteq B \setminus C\)
  - Proof:
    - \((\Rightarrow)\): Suppose \(x \in A \setminus C\). Then we know, from \(A \cup C\) that \(x \in B \cup C\). Now, either \(x \in B\) or \(x \in C\). We already know that \(x \notin C\). Hence, \(x \in B \setminus C\). Thus, \(    A \setminus C \subseteq B \setminus C\)
    - The converse is similar.
- 7
  - Goal: Let \(A::Set\) and \(B::Set\). \(\mathcal{P}(A) \cup \mathcal{P}(B) \subseteq \mathcal{P}(A\cup B)\).
  - Proof
    - Case 1 : \(x \in \mathcal{P}(A) \). Then \(x \subseteq A\). Hence, for any \(a \in x\) we know that it \(a \in A \cup B\). Since a is arbitrary it follows that x \(\subseteq A \cup B = x \in \mathcal{P}(A \cup B)\).
  - Case 2 is identical
- 10
  - Goal: \(|x - 3| > 3 \\to x^2 > 6x \)
  - Case 1:
    - Suppose \(|x-3| = x-3\). Then \(x-3 > 3 \to x >6 \to x^2 > 6x\)
  - Case 2:
    - Suppose \(|x - 3| = 3 - x \). Then \(3-x > 3 \to x < 0 \to x^2 > 0 \to x^2 > 6x\)
- 13
  - Let x even and let x odd and prove separately through substitution
** Section 3.6
- 2
  - Goal: \(\forall x \in \mathbb{R} \exists y (x^2y = x - y)\)
  - Proof:
    - (Existence): Let \(y = {x \over {x^2 + 1}}\). Then
      \[\begin{aligned}
      x - y = \\
      x - {x \over {x^2 + 1 }} = \\
      {{x^3 + x - x} \over {x^2 + 1}} = \\
      {{x^3}  \over {x^2 + 1 }} = \\
      x^2 {x \over {x^2 + 1}} = \\
      x^2 y
      \end{aligned} \]
    - (Uniqueness). Let \(x^2z = x -z \). Then
      \[
      x^2z = x -z \iff
       x^2z + z = x
       \\  \iff \\
        z(x^2 + 1) = x
        \\  \iff \\
        z = {x \over {x^2 + 1}}
         = y
        \]
- 3
  - Goal : \(\forall x \exists ! y(x \neq 0 \land x \neq 1 \to \frac{y}{x}  = y - x )\)
  - Proof :
    - (Existence): Let \(y = \frac{x^2}{x-1}\). Then we have that
      \[\begin{aligned}
      y - x = \\
      {x^2 \over {x-1} } - x = \\
      {x \over {x - 1}} = \\
      {x^2 \over {x^2 - x}} = \\
      {x^2 \over {x - 1}} {1 \over x} = \\
      {{x^2 \over {x-1}} \over x} = \\
      {y \over x}
      \end{aligned}\]
    - (Uniqueness) Same logic of exercise 1. Find that through algebraic manipulation \(z = y\).
- 4:
  - Goal : \(\forall x ( x \neq 0 \to \exists y \forall z (zy = {z \over x}))\)
  - Proof : easy, same as inchmeal.io proof
    - (Existence)
    - (Uniqueness)
- 5:
  a.
     - Goal: \(\cup!\mathcal{F} \subseteq \cup \mathcal{F}\)
       - Easy peasy. Suppose \(x \in \cup!\mathcal{F}\). Then there is an \(A_0 \in \mathcal{F} \) s.t. \(x \in A_0\). From that we already know that \(x \in \mathcal{F}\). Since x is arbitrary it follows that  \(\cup!\mathcal{F} \subseteq \cup \mathcal{F}\).
  b.
     - Bored
- 6:
  a. A = \(\emptyset\)
  b. A = U
- 7:
  a. U
  b. \(\emptyset\)
- 8:
  a. \(U \setminus A\)
  b. \(U \setminus A\)
- 9:
  a. \(\emptyset\)
  b. \(A\)
  c. \(A \triangle B\)
  d. A
- 10: TODO
- 11: TODO
- 12: TODO



** Section 4.1
- 5
  - Goal: \(A \times (B \cup C) = (A \times B ) \cup (A \times C) \)
  - Proof:
    - \( (\rightarrow)\) Suppose \((x,y) \in A \times (B \cup C)\) . Then \(x \in A\) and \(y \in B \cup C \) . We have two cases now. Let \(y \in B\)  (Case 1). Then \((x,y) \in A \times B\). Hence \((x,y) \in (A \times B ) \cup (A \times C) \) . Now let \(y \in C\)  (Case 2). Then \((x,y) \in A \times C\). Hence \((x,y) \in (A \times B ) \cup (A \times C) \). Therefore, \(A \times (B \cup C) \subseteq (A \times B ) \cup (A \times C) \)
    - \( (\leftarrow)\) Suppose \((x,y) \in (A \times B ) \cup (A \times C)\). We know have two cases. (Case 1) Let \((x,y) \in A \times B\) . Then \(y \in B \) and \(y \in B \cup C\) . It follows that \((x,y) \in A \times (B \cup C)\) . Case 2 is similar.
- 8
  - Goal: Prove or disprove \( A \times (B\setminus C) = (A \times B) \setminus (A \times C)\)
    - Its true. \[\begin{aligned}
      (x,y) \in  (A \times B) \setminus (A \times C)
      \iff \\
            x \in A \land y \in B \land (x \notin A \lor y \notin C) \iff
            \\
      x \in A  (x \notin A \lor y \notin C) \land y \in B  \; & \{\text{associativity of} \land \} \iff \\
        [(x \in A \land x \notin A) \lor (x \in \land y \notin C)] \land y \in B
        \; & \{\text{ distributivity of } \land\} \iff \\
      x \in A \land y \not \in C \land y \in B
     \; &  \{\text{distributivity of } \lor \text{ and contradiction law  }\} \iff \\ (x,y) \in A \times (B \setminus C)
      \end{aligned}\]

- 9
  - Goal : \(\forall A,B,C ((A \times B) \setminus (C \times D) = [A \times (B \setminus D)] \cup [(A \setminus C) \times B])\)
  - Proof:
     \[\begin{aligned}
    \text{ let x } = (a,b) \\
    x \in (A \times B) \setminus (C \times D) \iff \\
    x \in (A \times B) \land  x \notin (C \times D) \iff \\
    (a \in A \land b \in B) \land \neg (a \in C \land b \in D)  \iff \\
    (a \in A \land b \in B) \land (a \notin C \lor b \notin D) \iff \\
    (a \in A \land b \in B \land b \notin D) \lor (a \in A \land a \notin C \land b \in B) \iff \\
    x \in [A \times (B \setminus D)] \cup [(A \setminus C) \times B])
     \end{aligned}\]

- 10
  - Goal: \((A \times B) \cap (C \times D) = \emptyset
     \to (A \cap C = \emptyset)  \lor (B \cap C = \emptyset)\)
  - Suppose \(A \cap C\) are not disjoint and the same for \(B \cap D\). Then there is an \(a_0 \in A \cap C \) and a \(b_0 \in B \cap D\). Consequently, \((a,b) \in A \times B\) and \((a,b) \in C \times D\), which is equivalent to saying that \((a,b) \in (A \times B) \cap (C \times D)\). Hence \((A \times B) \cap (C \times D) \neq \emptyset\). Since \((a,b) \) is arbitrary:
      \((A \times B) \cap (C \times D) = \emptyset
     \to (A \cap C = \emptyset)  \lor (B \cap C = \emptyset)\)
- 11
  a. Goal:
     \(\cup_{i \in I}(A_i \times B_i) \subseteq (\cup_{i \in I}A_i) \times (\cup_{i \in I}B_i)\).
     - Suppose \((a,b) \in \cup_{i \in I}(A_i \times B_i)\). Then there is an \(i \in I \) s.t. \((a,b) \in A_i \times B_i\). Since \(a \in A_i\) we know that \(a \in  \cup_{i \in I} A\). Analogously for \(b\). Hence, \((a,b) \in (\cup_{i \in I}B_i)\).



  b. It is only the other side of the iff. Or a string of equivalences.



** Section 4.2
- 6
  - a
    - Goal: \(\text{Ran}(R^{-1}) = \text{Dom}(R) \)
      + Proof: Let \( (a,b) \in R\). Then \(\text{Dom}(R) = \{a \in A \; | \,  \exists b \in B ((a,b) \in R)\} = \{a \in A \; | \,  \exists b \in B ((b,a) \in R^{-1})\} = Ran(R^{-1}) \)
  - c
    - Goal : \(T \circ (S \circ R) = (T \circ S) \circ R\)
    - Proof:
      - Let :
        - \( R \subseteq A \times B\)
        - \( S \subseteq B \times C\)
        - \( T \subseteq C \times D\)
      - \[\begin{aligned}T \circ (S \circ R) = \\
         {(a,d) \in A \times D | \exists c \in C( (a,c) \in A \times C ( \exists b \in B ((a,b) \in A \times B) \text{ and } (b,c) \in B \times C) \text{ and } (c,d) \in C \times D)) = \\
         {(a,d) \in A \times D | \exists c \in C \exists b \in B( (a,c) \in A \times C  \text{ and }    (a,b) \in A \times B \text{ and } (b,c) \in B \times C \text{ and } (c,d) \in C \times D))  = \\
         {(a,d) \in A \times D |  \exists b \in B(  (a,b) \in R \text{ and } (b,d) \in T \circ S))            = \\
         (T \circ S) \circ R         \]
      - Now, a proper proof.
        - \((\rightarrow)\) Suppose \( (a,d) \in T \circ (S \circ R)  \). Then there is an \(c \in C\)  s.t. \(  (a,c) \in S \circ R \) and \( (c,d) \in T \). Since \( (a,c) \in S\circ R \) it follows that there is a \(b \in B\) s.t. \( (a,b) \in R \) and \( (b,c) \in S  \) . If \( (b,c) \in S \) and \( (c,d) \in T  \) , then \( (b,d) \in (T \circ S) \) . If \( (b,d) \in (T \circ S) \) and \( (a,b) \in R  \) it follows that \( (a,d) \in (T \circ S ) \circ   R \). Thus, if \( (a,d) \in T \circ (S \circ R)  \) then \( (a,d) \in (T \circ S ) \circ   R \).
        - \( (\leftarrow) \) Suppose \( (a,d) \in (T \circ S) \circ R \). then there is an \(b \in B \)  s.t. \( (b,d) \in (T \circ S) \) and \( (a,b) \in R \). If \( (b,d) \in (T \circ S) \), then there is a \(c \in C\) s.t. \( (b,c) \in S \) and \( (c,d) \in T \). if \( (a,b)  \in R \) and \( (b,c) \in S \) then \( (a,c) \in (S \circ R) \). From \( (a,c) \in (S \circ R) \)  and \( (c,d) \in T \) it follows that \( (a,d) \in T \circ (S \circ R) \) . Thus if \( (a,d) \in (T \circ S) \circ R \) then  \( (a,d) \in T \circ (S \circ R) \).


  - d :
    - Goal : \((S \circ R)^{-1} = R^{-1} \circ S^{-1}\)
    - Proof:
      - (\(\rightarrow\))  Suppose \( (c,a) \in (S \circ R )^{-1} \). then \( (a,c) \in S \circ R \). From that we know there is a \(b\) s.t. \( (a,b) \in R \) and \(  (b,c) \in S \).  Naturally, \( (b,a) \in R^{-1} \) and \( (c,b) \in S^{-1} \). Finally, if \( (b,a) \in R^{-1} \) and \( (c,a) \in R^{-1} \circ S^{-1}  \).
      - (\(\leftarrow\)) Suppose \( (c,a) \in R^{-1} \circ S^{-1} \). Then there is a \(b\) s.t. \( (b,a) \in R^{-1} \) and \( (c,b) \in S^{-1} \). Thus \( (a,b) \in R \) and \( (b,c) \in S^{-1} \). Thus \( (a,b) \in R \) and \( (b,c) \in S \). Clearly, \(  (a,c) \in S \circ R \). Finally, we can infer from \( (a,c) \in S \circ R  \) that \( (c,a) \in (S\circ R)^{-1}  \). Thus, if \( (c,a) \in R^{-1} \circ S^{-1} \), then \( (c,a) \in (S\circ R)^{-1} \).

- 8 :
  a. Goal: \(\text{Dom}(S \circ R) \subseteq \text{Dom}(R)\)
    -  Proof: Suppose \(a \in \text{Dom}(S\circ R)\). Then there is a \(c\) s.t.
      \((a,c) \in S \circ R\) , from which we infer that there is a \(b\) s.t.
      \(aRb\) and \(bSc\). Since \((a,b) \in R\) it follows that \(a \in
      \text{Dom}(R)\).Thus \(\text{Dom}(S \circ R) \subset \text{Dom}(R)\)
  b. We already know that \(\text{Dom}(S \circ R) \subseteq \text{Dom}(R)\). So, supoose \(a\in \text{Dom}(R)\). Then there is a \(b\) s.t. \(aRb\), from which can be inferred that \(b \in \text{Ran}(R)\). From \(\text{Ran}(R) \subseteq \text{Dom}(S)\)  it follows that \(b \in \text{Dom}(S)\). If \(b \in \text{Dom}(S)\), then there is a \(c\) s.t. \((b,c) \in S\) . So, \((a,c) \in (S \circ R)\). From that it is implied  that \(a \in \text{Dom}(S \circ R)\). thus, if \(a \in \text{Dom}(R)\) and \(\text{Ran}(R) \subseteq \text{Dom}(S)\) then  \(a \in \text{Dom}(S \circ R)\). All in all, \(\text{Ran}(R) \subseteq \text{Dom}(S)\) then  \(\text{Dom}(S \circ R) \subseteq \text{Dom}(R)\).

- 9:
  + a) true and easy to prove.
  + b) Suppose \(R \subseteq S\) Now suppose \((b,a) \in R^{-1}\) then \((a,b) \in R  \) then \((a,b) \in S\) then \((b,a) \in S^{-1}\).
  + c)
    - (\(\Rightarrow\)) Suppose \((b,a) \in  (R \cup S)^{-1} \iff (a,b) \in R \cup S \)
      - Case 1: \((a,b) \in R\) then \((b,a) \in R^{-1} \to (b,a) \in R^{-1} \cup S^{-1}\)
      - Case 2: The same for \(S\)
    -((\(\Leftarrow\)) Also case based
- 10
  - Interesting, I have to show that there is no \(b\). Too lazy now.



** Section 4.3
- 4
  - a: none
  - b: transitive
    + (a,b), (a,d)
    + (b,a), (b,d)
  - c: symmetric, reflexive and transitive
  - d: transitive
- 6 ???

- 7:
  - Goal: R is reflexive iff \(i_A \subseteq R\)
  - Proof:
    - \((\rightarrow) \) Suppose R is reflexive. Now suppose \((x,y) \in i_A\). Then  \(x = y \in A \). Using the reflexivity \((x,y) \in R\). Since \((x,y)\) was arbitrary \(i_A \subseteq R\).
    - \((\leftarrow)\) Similar.
- 8:
  - Goal: R is transitive iff \(R \circ R \subseteq R\)
  - Proof:
    - \((\rightarrow)\) Suppose R is transitive. Now suppose \((x,z) \in R \circ
      R\). Then there is a \(y_0 \in A\) s.t. \(xRy_0\) and \(y_0Rz\). From the
      transitivity it follows that \(xRz\). Since \((x,z)\) was arbitrary we
      have that \(R \circ R \subseteq R\)
    - \((\leftarrow)\) Suppose \(R \circ R \subseteq R\). Now suppose \(xRy\)
      and \(yRz\) . Since \(y \in A\) we have that \((x,z) \in R \circ R\) and ,
      from \(R \circ R \subseteq R\) , \((x,z) \in R\). Hence R is transitive.
- 9:
  - a) Goal: Let \(R \subseteq A \times B\), \(R \circ i_A = R\)
    - Proof (i was too lazy to prove it correctly. easy if split )
       \((a,b) \in R \circ i_A \iff ((a,b) \in A \times B \; | \; \exists c \in A ((a,c) \in i_A \text{ and } (c,b) \in R) \iff ((a,b) \in A \times b | \; (\exists c (c=a (a,a \in i_A \text{ and } (a,b) \in R)))  \iff a,b \in R \)
  - b) analogous. Ok lets do it properly (kinda). Goal: \(i_B \circ R = R \)
    - \((\leftarrow)\)  Suppose \((a,c) \in R\). Then \(c \in B \to (c,c) \in i_B \to a,c \in i_B \circ R\)
    - \((\rightarrow)\) Suppose \(a,c \in i_B \circ R \). Then there is a \(b
      \in B \) s.t. \(a,b \in R\) and \(b,c \in i_B\). From \(b,c \in i_B\) we
      know that \(b =c\) . Hence \(a,c \in R \)

- 10
  - Suppose \((a,a) \in i_D\). Then \(a \in D\). Then there is a \(b \in A\) s.t. \( (a,b) \in S \). Naturally, \((b,a) \in S^{-1}\). Then \((a,a) \in S^{-1} \circ S\).
  - Suppose \((b,b) \in i_R\). Then \(b \in \text{Ran}(S)\). Then there is an \(a \in A\) s.t. \((a,b) \in S\). Then \((b,a) \in S^{-1}\). Then \((b,b) \in S \circ S^{1}\) .
- 11
  - Suppose \((x,y) \in R\). Then \((x,x) \in R\). If \((x,y) \in R\) and \((x,x) \in R\) then \((x,y) \in R \circ R\). Thus \(R \subseteq R \circ R\).
- 12
  a. Let \(xRx\). Then \((x,x) \in R^{-1}\). Then \(R^{-1}\) is reflexive.
  b. Let \(R\) be symmetric and suppose \((x,y) \in R\). Then \((y,x) \in R\). From  the former that it follows that \( (y,x) \in R^{-1}\), while from the latter it follows that \((x,y) \in R^{-1}\). Thus, \(R^{-1}\) is symmetric
  c. Suppose \(R\) is transitive, and \(xRy\) and \(yRz\) . Naturally, \(xRz\). We now have that \((z,x) \in R^{-1}\), \((z,y) \in R^{-1}\) and \((y,x) \in R^{-1}\). Thus, \(R^{-1}\) is transitive

- 13

  a. Suppose \(a \in A \). Then we know that \(a,a \in R_1\). thus \(a,a \in R_1 \cup R_2\), which means \(R1 \cup R2\) is also reflexive
  b. Suppose \((x,y) \in R_1 \cup R_2\). Let \((x,y) \not \in R_1\). Then \((x,y) \in R_2\). Iit follows that \( (y,x) \in R_2\), which means that \((y,x) \in R_1 \cup R_2\). Thus \(R_1 \cup R2 \) is symmetric
  c. Suppose \((x,y) \) and \((y,z)\) are elements of \(R_1 \cup R2 \). It may
     be possible that \((x,y) \in R_1 \setminus R_2\) while \((y,z) \in R_2
     \setminus R_1\). So, we cannot affirm that \(R_1 \cup R_2\) will also be
     transitive. It will only be in some cases, not in all of them.


- 15
  - a) False. If R1 is reflexive but R2 is only the identity, then the elements that are in R1 will be in the R1 \ R2, but the set will not be reflexive.
  - b) R1 = {(0,0), (0,1), (1,0), (1,1)}
       R2 = {(1,1)}
       Seems true
  - c) Seems false.
- 16: x in A then x,x in R and x,x in S then x,x in R \(\circ\) S
- 17:
  - Given: \(R\) and \(S\) are symmetric on \(A\).
  - Goal: \(\text{Symm}(R \circ S) = \text{TRUE} \iff R\circ S = S  \circ R\)
  - Proof:
    - \((\rightarrow)\) Suppose \(\text{Symm}(R \circ S) = \text{TRUE}\).
      + Suppose \((a,c) \in R \circ S\). Since it is symmetric \((c,a) \in R \circ S \)
        - Then there is a \(b \in A\) s. t. \((a,b) \in S \) and \( (b,c) \in R\).
        - There is a \(d \in A \) s.t. \((d,a) \in R \)  and \((c,d) \in S\) .
        - \((a,b) \in S \) and \( (d,a) \in R \)  then \((d,b) \in  S \circ R\)
        - If \((c,d) \in S\) and \( (b,c) \in R\)  then \((d,c) \in S\) and \((c,b) \in R\) from which we know that \((d,b) \in R \circ S\)
        - The argument for \(S\circ R\) is almost identical
  - \((\leftarrow)\) Too lazy
- TODO 18:
  - Given: R and S are transitive on \(A\)
  - Goal: \(S \circ R \subseteq R \circ S \rightarrow R \circ S \text{ is transitive }\)
  - Proof:
    - Suppose \(R \circ S \) is not transitive. Then there is some \(x,y,z \in A\) in which \(x,y \in R \circ S\) and \(y,z \in R\circ S\) and \(x,z \notin R\circ S\) .

    - Now suppose \(a,c \in S \circ R\). Then there is a \(b \in A ( (a,b) \in R \text{ and }  (b,c) \in S)\)
    - \(x,y \in R \circ S \rightarrow \exists w \in A ((x,w) \in S \text{ and } (w,y) \in R)\)
    - \(y,z \in R \circ S \rightarrow \exists k \in A ((y,k) \in S \text{ and } (k,z) \in R)\)
    - \(x,z \notin R\circ S \to \forall m \in A ((x,m) \notin S \lor (m,z) \notin R)\)
- 19
  - Incorrect assumption that y is the same in different pairs
- 20
  - Suppose R is transitive. Now suppose \((X,Y) \in S\) and \((Y,Z) \in S\). For that we needed \(Y \in B\) where \(B \neq \emptyset\). Then we know that \(xRy\) and \(yRz\) . Since \(R\) is transitive we know that \(xRz\). Since x and z are arbitrary elements of X,Z it follows that \(XSZ\), but then \(S\) is transitive too.

- 21 TODO
- 22 TODO
- 23 TODO


** What are the laws of conjunction/disjunction? :fc:
:PROPERTIES:
:FC_CREATED: 2021-01-04T21:19:54Z
:FC_TYPE:  normal
:ID:       c692adcd-b1cf-4bb7-9e3c-bb82fa4e191d
:END:
:REVIEW_DATA:
| position | ease | box | interval | due                  |
|----------+------+-----+----------+----------------------|
| front    |  2.5 |   0 |        0 | 2021-01-04T21:19:54Z |
:END:

*** Back :ATTACH:

[[attachment:_20210104_182005screenshot.png]]
** How does one translate from logic to sets? :fc:
:PROPERTIES:
:FC_CREATED: 2021-01-04T22:27:35Z
:FC_TYPE:  normal
:ID:       8f7810e1-4dcd-463c-8bc6-ea32c64c9d3b
:END:
:REVIEW_DATA:
| position | ease | box | interval | due                  |
|----------+------+-----+----------+----------------------|
| front    |  2.5 |   0 |        0 | 2021-01-04T22:27:35Z |
:END:

*** Back :ATTACH:
By using *truth sets*

[[attachment:_20210104_192750screenshot.png]]
]



Essa noite tive um sonho q pra mim foi bem engracado. Eu tava numa festa do ensino medio. Tinha nocao q tava bem bebado. Ai na primeira parte eu tava num telhado, sentado na beira, conversando com chico e outra pessoa. Ai eu descia pq tava com vertigem. Desci flutuando (????). Ai eu tentava conversar embaixo, mas a voz de chico tava bem baixa. Quando olho pra cima ele tinha encolhido e tava falando de dentro de um sapato (????????). Ai eu desistia. Depois em outra parte eu ia perguntar a Isabella se eu podia entrar na justica pra n ter q terminar o ensino medio pq afinal eu ja tinha diploma de graduacao e mestrado KKKKKK E ela falava q achava q sim kkkkk Sendo q Vinicius tava junto ai ele falava : "Porra, ote f√©, vou entrar tbm " KKKKKKK ai eu me tocava q era chapacao minha e vinicius chapado entrou na noia, ai eu tinha uma crise de riso gigante no sonho. Ai acordei.
